src/coqutil/Map/SortedListString_test.v
@@ -1,14 +1,15 @@
 Require Import coqutil.Map.Interface Coq.Strings.String.
 Require coqutil.Map.SortedListString.
-Local Existing Instance SortedListString.map.
+Require Import coqutil.Macros.ElpiRecordImport.
 Local Open Scope string_scope. Local Open Scope list_scope.
-Local Existing Instance SortedListString.map.
-
+Require Import coqutil.Macros.ElpiRecordImport.
 Import SortedList List.ListNotations.
+import.projections (SortedListString.map nat).
+
 Goal False.
-  assert (value (map.put (map.put (map.put map.empty "a" 6) "z" 0) "c" 9) = [("a", 6); ("c", 9); ("z", 0)]%list) by exact eq_refl.
-  assert ((map.get (map.put (map.put (map.put map.empty "a" 6) "z" 0) "c" 9) "c") = Some 9) by exact eq_refl.
-  assert ((map.get (map.put (map.put (map.put map.empty "a" 6) "z" 0) "c" 9) "z") = Some 0) by exact eq_refl.
-  assert ((map.get (map.put (map.put (map.put map.empty "a" 6) "z" 0) "c" 9) "x") = None) by exact eq_refl.
-  assert (map.putmany (map.put (map.put map.empty "z" 7) "0" 0) (map.put (map.put (map.put map.empty "a" 6) "z" 0) "c" 9) = (map.put (map.put (map.put (map.put map.empty "a" 6) "z" 0) "c" 9) "0" 0)) by exact eq_refl.
+  assert (value (put (put (put empty "a" 6) "z" 0) "c" 9) = [("a", 6); ("c", 9); ("z", 0)]%list) by exact eq_refl.
+  assert ((get (put (put (put empty "a" 6) "z" 0) "c" 9) "c") = Some 9) by exact eq_refl.
+  assert ((get (put (put (put empty "a" 6) "z" 0) "c" 9) "z") = Some 0) by exact eq_refl.
+  assert ((get (put (put (put empty "a" 6) "z" 0) "c" 9) "x") = None) by exact eq_refl.
+  assert (map.putmany (put (put empty "z" 7) "0" 0) (put (put (put empty "a" 6) "z" 0) "c" 9) = (put (put (put (put empty "a" 6) "z" 0) "c" 9) "0" 0)) by exact eq_refl.
 Abort.
